

**DS & AI
CS & IT**

Linear Algebra

Lecture No. 09



By- Dr. Puneet Sharma Sir

Recap of previous lecture



Topic

EIGEN VALUES & their properties




Topics to be Covered



Topic

- (1) CAYLEY-HAMILTON THEOREM
- (2) Methods of finding Eigen Vectors



Cayley-Hamilton Theorem → "Every square Mat satisfies it's own C-Eq." 
ie we can Replace $\lambda \rightarrow A$ in C-Eq.

Consider $A_{n \times n}$ then it's C-Eq is $|A - \lambda I| = 0$

$$\lambda^n + a_1 \lambda^{n-1} + a_2 \lambda^{n-2} + \dots + a_{n-1} \lambda + a_n = 0 \longrightarrow \text{Algebraic Eqn}$$

Using C.H.T, $\lambda \rightarrow A$

$$1. A^n + a_1 A^{n-1} + a_2 A^{n-2} + \dots + a_{n-1} A + a_n I = 0 \longrightarrow \text{Matrix Eqn}$$

Application: with the help of C.H.T we can calculate $\text{Tr}(A)$, $|A|$, A^{-1} & A^n = ?

$$(1) \text{Tr}(A) = -(a_1)$$

$$(2) |A| = (-1)^n a_n$$

$$(3) A^{-1} = \text{will be discussed in Questions}$$

$$(4) A^n = \text{" " " " " "}$$

Take Care: Above Results are Valid when Coeff of $A^n = 1$

Some More Conclusions from C.H.T.:-



① Constant term in the C-Eq of $A_{n \times n} = a_n = \begin{cases} -|A|, & n = \text{odd} \\ +|A|, & n = \text{even} \end{cases}$

Proof: we know that (by C.H.T)

$$|A| = (-1)^n a_n$$

$$(-1)^n |A| = (-1)^n \cdot (-1)^n a_n$$

$$(-1)^n |A| = (-1)^{2n} a_n$$

$$(-1)^{2n} a_n = (-1)^n |A|$$

ie $a_n = (-1)^n |A| = \begin{cases} -|A|, & n = \text{odd} \\ +|A|, & n = \text{even} \end{cases}$

② Shortcut Method of finding C-Eq of $A_{2 \times 2}$

C-Equⁿ is $|A - \lambda I| = 0$

$$\lambda^2 + a_1 \lambda + a_2 = 0$$

$$\lambda^2 - (-a_1) \lambda + \{(-1)^2 a_2\} = 0$$

$$\lambda^2 - (\text{Tr } A) \lambda + (|A|) = 0$$

Q for the Matrix $A = \begin{bmatrix} 2 & 1 & 1 \\ 1 & 2 & 1 \\ 0 & 0 & 1 \end{bmatrix}$ Evaluate $\text{Tr}(A)$, $|A|$, & A^{-1} ? using C.H.Th.



Sol C-Equⁿ of A is $|A - \lambda I| = 0$

$$(\lambda - 3)(\lambda - 1)^2 = 0$$

$$\lambda^3 - 5\lambda^2 + 7\lambda - 3 = 0$$

By C.H.Th, $\lambda \rightarrow A$

$$\boxed{A^3 - 5A^2 + 7A - 3I = 0} \quad \text{--- (1)}$$

on comparison with,

$$A^3 + a_1 A^2 + a_2 A + a_3 I = 0$$

$$\textcircled{1} \text{Tr}(A) = -(a_1) = -(-5) = +5 \quad \checkmark$$

$$\textcircled{2} |A| = (-1)^3 a_3 = -(-3) = +3 \quad \checkmark$$

$\textcircled{3} \because |A| \neq 0$ ie A^{-1} exist. So By (1),

$$A^{-1}(A^3 - 5A^2 + 7A - 3I) = A^{-1} \cdot 0$$

$$A^2 - 5A + 7I - 3A^{-1} \cdot I = 0$$

$$-3A^{-1} = -(A^2 - 5A + 7I)$$

$$A^{-1} = \frac{1}{3}(A^2 - 5A + 7I) \quad \underline{\underline{Ans}}$$

(iv) Evaluate $B = A^8 - 5A^7 + 7A^6 - 3A^5 + A^4 - 5A^3 + 7A^2 + 4A + 2I = ?$

By (i) we know that
 $A^3 - 5A^2 + 7A - 3I = 0$ ①

$$B = A^5(A^3 - 5A^2 + 7A - 3I) + A(A^3 - 5A^2 + 7A - 3I) + 7A + 2I$$

$$= A^5(O) + A(O) + 7A + 2I$$

$$B = 7A + 2I$$

(a) $A+2I$ (b) $2I$

☒ (c) $7A+2I$ (d) O

(ii) Also Evaluate $|B| = ? = |7A + 2I| = \cancel{7|A| + 2|I|} = \cancel{7(3) + 2(1)} = \cancel{23}$

$$B = 7A + 2I = 7 \begin{bmatrix} 2 & 1 & 1 \\ 1 & 2 & 1 \\ 0 & 0 & 1 \end{bmatrix} + 2 \begin{bmatrix} 1 & 0 & 0 \\ 0 & 1 & 0 \\ 0 & 0 & 1 \end{bmatrix} = \begin{bmatrix} 16 & 7 & 7 \\ 7 & 16 & 7 \\ 0 & 0 & 9 \end{bmatrix}$$

$$|B| = 9[256 - 49] = 9 \times 207 = 1863$$

Q. If $P_{3 \times 3}$ Mat. s.t. it is C.Eq in $a(\lambda) = |\lambda I - P| = \lambda^3 + \lambda^2 + \lambda + 1 = 0$
 then evaluate $\text{Tr}(P)$, $|P|$, P^{-1}

Sol: C.Eqⁿ of P is $|P - \lambda I| = 0$

$$(-1)^3 |\lambda I - P| = 0$$

$$|\lambda I - P| = 0$$

$$\lambda^3 + \lambda^2 + \lambda + 1 = 0$$

By C.H.T, $\lambda \rightarrow P$

$$P^3 + P^2 + P + I = 0 \quad \text{--- (1)}$$

on comparison with, $(P^3 + a_1 P^2 + a_2 P + a_3 I = 0)$

$$(i) \text{Tr}(P) = -(a_1) = -(1) = -1$$

$$(ii) |P| = (-1)^3 a_3 = -(1) = -1$$

$$(iii) \text{By (1), } P^{-1}(P^3 + P^2 + P + I) = P^{-1} \cdot 0$$

$$P^2 + P + I + P^{-1} = 0$$

$$P^{-1} = -(P^2 + P + I)$$

(iv) if $B = P^8 + P^7 + P^6 + P^5 + P^4 + P^3 + P^2 + P + 4I$ then $|B| = ?$

(a) 1 $= P^5(P^3 + P^2 + P + I) + P(P^3 + P^2 + P + I) + 4I$

(b) -1 $B = P^5(0) + P(0) + 4I$

(c) 4 $B = 4I \Rightarrow |B| = |4I| = 4^3 |I| = 64(1) = 64$

~~(d) 64~~

Q₁ Evaluate the constant term in the C.Eqnⁿ of $A = \begin{bmatrix} 2 & 1 & 1 & 1 \\ 1 & 2 & 1 & 1 \\ 1 & 1 & 2 & 1 \\ 1 & 1 & 1 & 2 \end{bmatrix}_{4 \times 4}$

(M-I) C.Eqnⁿ is $|A - \lambda I| = 0$

$$\begin{vmatrix} (2-\lambda) & 1 & 1 & 1 \\ 1 & (2-\lambda) & 1 & 1 \\ 1 & 1 & (2-\lambda) & 1 \\ 1 & 1 & 1 & (2-\lambda) \end{vmatrix} = 0$$

$$\lambda^4 - 8\lambda^3 + a_2\lambda^2 + a_3\lambda + (5) = 0$$

So constant term = 5 Ans

(M-II) $|A| = \dots = 5$

'A' is of even order so

$$a_n = (-1)^4 |A| = +|A| = +5 \quad \underline{\underline{Ans}}$$

Q₂ Constant term in the C.Eqn of $\begin{bmatrix} 0 & 1 & 2 & -3 & 4 \\ -1 & 0 & 4 & -1 & 2 \\ -2 & -4 & 0 & 3 & 0 \\ 3 & 1 & -3 & 0 & 2 \\ -4 & -2 & 3 & 0 & -2 \end{bmatrix}$

'A' is Skew Symm Mat of odd order

So $|A| = 0 \Rightarrow$ const term $a_5 = -|A| = 0$ ^{5x5}

Q If $A = \begin{bmatrix} -1 & -2 \\ 0 & 3 \end{bmatrix}$ then A will satisfy ?

(a) $A^2 - 2A - 3I$

(b) $(A+I)(A-3I) = 0$

(c) $A - 2I - 3A^{-1} = 0$

(d) $A^2 - 3A + 2I = 0$

C-Equⁿ of A is $|A - \lambda I| = 0$

$$\lambda^2 - (\text{Tr}(A))\lambda + |A| = 0$$

$$\lambda^2 - (2)\lambda + (-3) = 0$$

By C-H-T, $A^2 - 2A - 3I = 0$ Ans

A^{-1}
 $A - 2I - 3A^{-1} = 0$
Ans

factor
 $(A+I)(A-3I) = 0$
Ans

TAG DAA QUEST:-

Q if $A = \begin{bmatrix} -1 & -2 \\ 0 & 3 \end{bmatrix}$ then which is/are true

(MSQ) (a) $A^2 - 2A - 3I$

(b) $(A - 3I)(A + I) = 0$

(c) $A - 2I - 3A^{-1}$

(d) $A^2 - 3A - 2I$

Q. If E-Values of $A_{4 \times 4}$ are ± 1 & $\pm i$ then $A^4 = ?$

- (a) A
- (b) O
- (c) I_3
- (d) I_4

$$\because \lambda = 1, -1, i, -i$$

So C-Equⁿ is

$$(\lambda - 1)(\lambda + 1)(\lambda - i)(\lambda + i) = 0$$

$$(\lambda^2 - 1)(\lambda^2 - i^2) = 0$$

$$(\lambda^2 - 1)(\lambda^2 + 1) = 0$$

$$(\lambda^4 - 1^2) = 0$$

$$\lambda^4 - 1 = 0$$

By C.H.Th, $\lambda \rightarrow A$

$$A^4 - I = O$$

$$A^4 - I = I_{4 \times 4} = I_4$$

Q: if CE of $A_{4 \times 4}$ is $\underline{2\lambda^4 - 6\lambda^3 + 4\lambda^2 - 8\lambda + 12 = 0}$ then $|A| = \underline{\hspace{2cm}}$

Ans: CE of A is $\lambda^4 - 3\lambda^3 + 2\lambda^2 - 4\lambda + 6 = 0$

So $|A| = (-1)^4 a_4 = (+1)(6) = 6$

Q: Constant term in the CE of $A = \begin{bmatrix} 0 & 1 & 2 & 3 \\ 1 & 0 & 3 & 0 \\ 2 & 3 & 0 & 1 \\ 3 & 0 & 1 & 2 \end{bmatrix}$ will be ?

(HW)

$\therefore |A| = \dots = \textcircled{88}$

So Constant term in CE of $A = a_n = (-1)^4 |A| = + (88)$

EIGEN VECTORS

Defⁿ! Consider Sq. Mat $A_{n \times n}$ then Non Zero Vector X is called Eigen Vector, corresponding to Eigen value λ (Real/Complex/Zero) if we are able to find a relationship of the type,

$$\boxed{AX = \lambda X}$$

$\swarrow \lambda = \text{Eigen Value}$
 $\searrow X = \text{Eigen Vector.}$

LHS is the Multi of Two Matrices = RHS is the Scalar Multi in a Mat

(Tough)
(Easy)

(*) Here we are considering Homogeneous system as follows

$$AX = \lambda X \Rightarrow AX - \lambda X = 0 \Rightarrow \boxed{(A - \lambda I)X = 0}$$

So it will satisfy all the prop of Homog system.

PROPERTIES of E-VECTORS →



① If x is an E-vector of A then (kx) will also be an E-vector

$$Ax = \lambda x$$

$$A(kx) = \lambda(kx)$$

$$(A - \lambda I)x = 0 \quad \text{E-vector}$$

$$k(A - \lambda I)x = k \cdot 0$$

$$(A - \lambda I)(kx) = 0 \quad \text{E-vector}$$

i.e. "we are free to multiply or divide with any constant in case of E-vector."

② E-Vectors corresponding to different E values of symm Mat are orthogonal

Q. if $A_{3 \times 3}$ s.t. $A^T = A$ ^{= symm.} and a, b are the E-Values & corresponding E-vectors are $\begin{bmatrix} x_1 \\ x_2 \\ x_3 \end{bmatrix}$ & $\begin{bmatrix} y_1 \\ y_2 \\ y_3 \end{bmatrix}$ then for $a \neq b$ the value of different E values

$$x_1 y_1 + x_2 y_2 + x_3 y_3 = \underline{\quad ? \quad}$$

By above property $X \cdot Y = 0 \Rightarrow X^T Y = 0$
 $\Rightarrow x_1 y_1 + x_2 y_2 + x_3 y_3 = 0$

- ③ For Different E-Values, Corresponding E-Vectors are also LI
- ④ If E-Value Repeats (then Headache will start) then Corresponding E Vectors may be LI or may be LD.
- ⑤ MODAL MATRIX: \rightarrow Matrix formed by E-Vectors is Called Modal Mat
- Let $A_{3 \times 3}$ is the given Mat & X_1, X_2, X_3 are the E-Vectors then
- Modal Mat is $P = [X_1 X_2 X_3]$

Ex: for $A = \begin{bmatrix} 4 & 2 \\ 2 & 4 \end{bmatrix}$ $\rightarrow \lambda = 6, X_1 = \begin{bmatrix} 1 \\ 1 \end{bmatrix} \because AX_1 = 6X_1$

$\searrow \lambda = 2, X_2 = \begin{bmatrix} -1 \\ 1 \end{bmatrix} \because AX_2 = 2X_2$

Now we try to understand the procedure of finding E-Vector.

Qs Find the E-Values & E-Vectors of $A = \begin{bmatrix} 4 & 2 \\ 2 & 4 \end{bmatrix}$

Sol: C-Equⁿ is $|A - \lambda I| = 0 \Rightarrow \lambda^2 - (8)\lambda + (12) = 0 \Rightarrow (\lambda - 6)(\lambda - 2) = 0 \Rightarrow \lambda = 6 \& 2$

Eigen Vector for $(\lambda = 6)$ \rightarrow

Consider $AX = \lambda X$

$$(A - \lambda I)X = 0$$

$$(A - 6I)X = 0$$

$$\begin{bmatrix} (4-6) & 2 \\ 2 & (4-6) \end{bmatrix} X = 0$$

$$\begin{bmatrix} -2 & 2 \\ 2 & -2 \end{bmatrix} X = 0$$

$$R_2 \rightarrow R_2 + R_1$$

$$\begin{bmatrix} -2 & 2 \\ 0 & 0 \end{bmatrix}_{2 \times 2} \begin{bmatrix} x_1 \\ x_2 \end{bmatrix}_{2 \times 1} = \begin{bmatrix} 0 \\ 0 \end{bmatrix}_{2 \times 1} \Rightarrow \begin{bmatrix} (-2x_1 + 2x_2) \\ 0 \end{bmatrix} = \begin{bmatrix} 0 \\ 0 \end{bmatrix}$$

$$\text{i.e. } \begin{cases} -2x_1 + 2x_2 = 0 \\ 0 = 0 \end{cases} \Rightarrow \boxed{x_1 = x_2} = k \text{ (let)}$$

$$X = \begin{bmatrix} x_1 \\ x_2 \end{bmatrix} = \begin{bmatrix} k \\ k \end{bmatrix} = k \begin{bmatrix} 1 \\ 1 \end{bmatrix}$$

E. Vector for $\lambda=2$ \rightarrow

Consider $AX = \lambda X$

$$(A - \lambda I)X = 0$$

$$(A - 2I)X = 0$$

$$\begin{bmatrix} 4-2 & 2 \\ 2 & 4-2 \end{bmatrix} X = 0$$

$$\begin{bmatrix} 2 & 2 \\ 2 & 2 \end{bmatrix} X = 0$$

$$R_2 \rightarrow R_2 - R_1 \quad \begin{bmatrix} 2 & 2 \\ 0 & 0 \end{bmatrix} \begin{bmatrix} x_1 \\ x_2 \end{bmatrix} = \begin{bmatrix} 0 \\ 0 \end{bmatrix}$$

$$\begin{bmatrix} 2x_1 + 2x_2 \\ 0 \end{bmatrix} = \begin{bmatrix} 0 \\ 0 \end{bmatrix}$$

$$\Rightarrow \begin{matrix} 2x_1 + 2x_2 = 0 \\ 0 = 0 \end{matrix} \Rightarrow x_1 = -x_2$$

Let $x_2 = k$ then $x_1 = -k$ so

$$X = \begin{bmatrix} x_1 \\ x_2 \end{bmatrix} = \begin{bmatrix} -k \\ k \end{bmatrix} = k \begin{bmatrix} -1 \\ 1 \end{bmatrix}$$

Finally, $A = \begin{bmatrix} 4 & 2 \\ 2 & 4 \end{bmatrix}$ $\begin{cases} \lambda = 6, X = \begin{bmatrix} 1 \\ 1 \end{bmatrix} \\ \lambda = 2, X = \begin{bmatrix} -1 \\ 1 \end{bmatrix} \end{cases}$

Analysis (PODCAST) →

① $A = \begin{bmatrix} 4 & 2 \\ 2 & 4 \end{bmatrix}$ $\swarrow \lambda=6, X_1 = \begin{bmatrix} 1 \\ 1 \end{bmatrix} \rightarrow \begin{bmatrix} 2 \\ 2 \end{bmatrix}, \begin{bmatrix} -3 \\ -3 \end{bmatrix}, \begin{bmatrix} 1/4 \\ 1/4 \end{bmatrix} \dots \infty$ E vectors exist.
 But all are LD on X_1

$\searrow \lambda=2, X_2 = \begin{bmatrix} -1 \\ 1 \end{bmatrix} \rightarrow \begin{bmatrix} -2 \\ 2 \end{bmatrix}, \begin{bmatrix} 1 \\ -1 \end{bmatrix}, \begin{bmatrix} 1/5 \\ -1/5 \end{bmatrix} \dots \infty$ E vectors exist.
 But all are LD on X_2

② Here X_1 & X_2 are LI (By observation)

Actually we are getting two Ind families of E. vectors. & if we are taking one member from F_1 & one member from F_2 then these are LI
 i.e for Mat A, ∃ two LI eigen vectors at a time

③ $A = \begin{bmatrix} 4 & 2 \\ 2 & 4 \end{bmatrix}$, $\begin{cases} \lambda = 6, \chi_1 = \begin{bmatrix} 1 \\ 1 \end{bmatrix} \\ \lambda = 2, \chi_2 = \begin{bmatrix} -1 \\ 1 \end{bmatrix} \end{cases}$ $\because \chi_1 \cdot \chi_2 = (1)(-1) + (1)(1) = 0$
 = Symm Mat.

i.e. χ_1 & χ_2 are orthogonal vectors \Rightarrow Hence they are LI also.
 i.e. for different eigen values of Symm Mat,
 corresponding E. vectors are orthogonal as well as LI.

④ In this Mat, $x_1 \cdot x_2 = \begin{bmatrix} -1 \\ 1 \end{bmatrix} \cdot \begin{bmatrix} 1 \\ 1 \end{bmatrix} = (-1)(1) + (1)(1) = 0$

is x_1 & x_2 are orthogonal Vectors.

⑤ one pair of L-I E vectors of $A = \begin{bmatrix} 4 & 2 \\ 2 & 4 \end{bmatrix}$ will be

(a) $\begin{bmatrix} -3 \\ 3 \end{bmatrix}, \begin{bmatrix} 4 \\ -4 \end{bmatrix}$

(b) $\begin{bmatrix} 3 \\ 3 \end{bmatrix}, \begin{bmatrix} -1 \\ -1 \end{bmatrix}$

(c) $\begin{bmatrix} -1 \\ 1 \end{bmatrix}, \begin{bmatrix} 2 \\ 3 \end{bmatrix}$

(d) $\begin{bmatrix} 3 \\ -3 \end{bmatrix}, \begin{bmatrix} 0.5 \\ 0.5 \end{bmatrix}$

Qs find E. Values & E. Vectors of $A = \begin{bmatrix} 1 & 2 \\ 0 & 2 \end{bmatrix}$

Sol: $\because A$ is U.T.M $\therefore \lambda = 1 \neq 2$

E. Vector for $\lambda = 1$ \rightarrow

$$AX = \lambda X$$

$$(A - \lambda I)X = 0$$

$$(A - I)X = 0$$

$$\begin{bmatrix} (1-1) & 2 \\ 0 & (2-1) \end{bmatrix} X = 0$$

$$\begin{bmatrix} 0 & 2 \\ 0 & 1 \end{bmatrix} X = 0$$

$$R_2 \rightarrow R_2 - \frac{1}{2} R_1; \begin{bmatrix} 0 & 2 \\ 0 & 0 \end{bmatrix} \begin{bmatrix} x_1 \\ x_2 \end{bmatrix} = \begin{bmatrix} 0 \\ 0 \end{bmatrix}$$

$$\begin{bmatrix} 2x_2 \\ 0 \end{bmatrix} = \begin{bmatrix} 0 \\ 0 \end{bmatrix} \Rightarrow x_2 = 0, \text{ let } x_1 = k$$

$$X = \begin{bmatrix} x_1 \\ x_2 \end{bmatrix} = \begin{bmatrix} k \\ 0 \end{bmatrix} = k \begin{bmatrix} 1 \\ 0 \end{bmatrix} \text{ i.e. for } \lambda = 1, X = \begin{bmatrix} 1 \\ 0 \end{bmatrix}$$

E. Vector for $\lambda=2$ \rightarrow

Consider $AX = \lambda X$

$$(A - \lambda I)X = 0$$

$$(A - 2I)X = 0$$

$$\begin{bmatrix} (1-2) & 2 \\ 0 & (2-2) \end{bmatrix} X = 0$$

$$\begin{bmatrix} -1 & 2 \\ 0 & 0 \end{bmatrix} \begin{bmatrix} x_1 \\ x_2 \end{bmatrix} = \begin{bmatrix} 0 \\ 0 \end{bmatrix}$$

$$\begin{bmatrix} (-x_1 + 2x_2) \\ 0 \end{bmatrix} = \begin{bmatrix} 0 \\ 0 \end{bmatrix}$$

$$\begin{cases} -x_1 + 2x_2 = 0 \\ 0 = 0 \end{cases} \Rightarrow x_1 = 2x_2$$

Let $x_2 = k$ then $x_1 = 2k$ so

$$X = \begin{bmatrix} x_1 \\ x_2 \end{bmatrix} = \begin{bmatrix} 2k \\ k \end{bmatrix} = k \begin{bmatrix} 2 \\ 1 \end{bmatrix}$$

so for $\lambda=2$, $X = \begin{bmatrix} 2 \\ 1 \end{bmatrix}$

finally $A = \begin{bmatrix} 1 & 2 \\ 0 & 2 \end{bmatrix} \begin{cases} \lambda=1, X = \begin{bmatrix} 1 \\ 0 \end{bmatrix} \\ \lambda=2, X = \begin{bmatrix} 2 \\ 1 \end{bmatrix} \end{cases}$

Q2 Find the E-Values and E-Vectors of $A = \begin{bmatrix} 2 & 1 & 0 \\ 0 & 2 & 0 \\ 0 & 0 & 3 \end{bmatrix}$

Sol: $\because A$ is U.T.M so $\lambda = 2, 2, 3$

E-Vector for $(\lambda=3)$ \rightarrow

$$AX = \lambda X$$

$$(A - \lambda I)X = 0$$

$$(A - 3I)X = 0$$

$$\begin{bmatrix} (2-3) & 1 & 0 \\ 0 & (2-3) & 0 \\ 0 & 0 & (3-3) \end{bmatrix} X = 0$$

$$\begin{bmatrix} -1 & 1 & 0 \\ 0 & -1 & 0 \\ 0 & 0 & 0 \end{bmatrix} X = 0$$

$$\begin{bmatrix} -1 & 1 & 0 \\ 0 & -1 & 0 \\ 0 & 0 & 0 \end{bmatrix} \begin{bmatrix} x_1 \\ x_2 \\ x_3 \end{bmatrix} = \begin{bmatrix} 0 \\ 0 \\ 0 \end{bmatrix}$$

$$\begin{bmatrix} (-x_1 + x_2) \\ -x_2 \\ 0 \end{bmatrix} = \begin{bmatrix} 0 \\ 0 \\ 0 \end{bmatrix} \Rightarrow \begin{matrix} -x_1 + x_2 = 0 \\ -x_2 = 0 \\ 0 = 0 \end{matrix}$$

ie $x_2 = 0$, $x_1 = x_2 = 0$ so $x_1 = 0$

let $x_3 = k$ so

$$X = \begin{bmatrix} x_1 \\ x_2 \\ x_3 \end{bmatrix} = \begin{bmatrix} 0 \\ 0 \\ k \end{bmatrix} = k \begin{bmatrix} 0 \\ 0 \\ 1 \end{bmatrix} \text{ ie for } \lambda=3, X = \begin{bmatrix} 0 \\ 0 \\ 1 \end{bmatrix}$$

E. Vector for $\lambda=2$ \rightarrow

Consider $AX = \lambda X$

$$(A - \lambda I)X = 0$$

$$(A - 2I)X = 0$$

$$\begin{bmatrix} (2-2) & 1 & 0 \\ 0 & (2-2) & 0 \\ 0 & 0 & (3-2) \end{bmatrix} X = 0$$

$$\begin{bmatrix} 0 & 1 & 0 \\ 0 & 0 & 0 \\ 0 & 0 & 1 \end{bmatrix} X = 0$$

$R_2 \leftrightarrow R_3$

$$\begin{bmatrix} 0 & 1 & 0 \\ 0 & 0 & 1 \\ 0 & 0 & 0 \end{bmatrix} \begin{bmatrix} x_1 \\ x_2 \\ x_3 \end{bmatrix} = \begin{bmatrix} 0 \\ 0 \\ 0 \end{bmatrix}$$

$$\begin{bmatrix} x_2 \\ x_3 \\ 0 \end{bmatrix} = \begin{bmatrix} 0 \\ 0 \\ 0 \end{bmatrix} \Rightarrow x_2 = 0, x_3 = 0$$

Let $x_1 = K$

$$X = \begin{bmatrix} x_1 \\ x_2 \\ x_3 \end{bmatrix} = \begin{bmatrix} K \\ 0 \\ 0 \end{bmatrix} = K \begin{bmatrix} 1 \\ 0 \\ 0 \end{bmatrix}$$

$$\text{So for } \lambda = 2, X = \begin{bmatrix} 1 \\ 0 \\ 0 \end{bmatrix}$$

finally:

$$A = \begin{bmatrix} 2 & 1 & 0 \\ 0 & 2 & 0 \\ 0 & 0 & 3 \end{bmatrix}$$

$(\lambda = 3, 2, 2)$

$$\lambda = 3, X = \begin{bmatrix} 0 \\ 0 \\ 1 \end{bmatrix}$$

$$\lambda = 2, X = \begin{bmatrix} 1 \\ 0 \\ 0 \end{bmatrix}$$

Qs Find E. Values & E Vectors of $A = \begin{bmatrix} 2 & 1 & 1 \\ 1 & 2 & 1 \\ 0 & 0 & 1 \end{bmatrix}$



Sol: Characteristic Eqn is $|A - \lambda I| = 0 \rightarrow (\lambda - 3)(\lambda - 1)^2 = 0 \Rightarrow \lambda = 3, 1, 1$

E. Vector for $\lambda = 3$

$$AX = \lambda X \\ (A - 3I)X = 0$$

(HW)

$$\text{for } \lambda = 3, X_1 = \begin{bmatrix} 1 \\ 1 \\ 0 \end{bmatrix}$$

E. Vector for $\lambda = 1$ \rightarrow

$$AX = \lambda X \\ (A - \lambda I)X = 0 \\ (A - I)X = 0$$

$$\begin{bmatrix} 1 & 1 & 1 \\ 1 & 1 & 1 \\ 0 & 0 & 0 \end{bmatrix} X = 0$$

$$\begin{bmatrix} 1 & 1 & 1 \\ 0 & 0 & 0 \\ 0 & 0 & 0 \end{bmatrix} \begin{bmatrix} x_1 \\ x_2 \\ x_3 \end{bmatrix} = \begin{bmatrix} 0 \\ 0 \\ 0 \end{bmatrix}$$

$$\begin{bmatrix} x_1 + x_2 + x_3 \\ 0 \\ 0 \end{bmatrix} = \begin{bmatrix} 0 \\ 0 \\ 0 \end{bmatrix} \Rightarrow x_1 + x_2 + x_3 = 0$$

Let $x_3 = k_1, x_2 = k_2$

$$x_1 = -(k_2 + k_1)$$

$$X = \begin{bmatrix} x_1 \\ x_2 \\ x_3 \end{bmatrix} = \begin{bmatrix} -(k_2 + k_1) \\ k_2 \\ k_1 \end{bmatrix}$$

$$X = \begin{bmatrix} -(K_2 + K_1) \\ K_2 \\ K_1 \end{bmatrix} = \begin{bmatrix} -K_2 \\ K_2 \\ 0 \end{bmatrix} + \begin{bmatrix} -K_1 \\ 0 \\ K_1 \end{bmatrix} = K_2 \begin{bmatrix} -1 \\ 1 \\ 0 \end{bmatrix} + K_1 \begin{bmatrix} -1 \\ 0 \\ 1 \end{bmatrix}$$

ie for $\lambda = 1$ we are getting two E-vectors $\begin{cases} X_2 = \begin{bmatrix} -1 \\ 1 \\ 0 \end{bmatrix} \because AX_2 = 1 \cdot X_2 \\ X_3 = \begin{bmatrix} -1 \\ 0 \\ 1 \end{bmatrix} \because AX_3 = 1 \cdot X_3 \end{cases}$

THANK - YOU

Tel:

dr puneet & pw